Progress on restoring Spec.ECIES

specs/Spec.ECIES.fst
@@ -6,140 +6,107 @@ open Lib.Sequence
 open Lib.ByteSequence
 
 
+module Hash = Spec.Hash
+
+
+
+(* BB. TODO: Relocate this function *)
 assume val crypto_random: len:size_nat -> Tot (lbytes len)
 
-
-(** Definition of a ECKEM IV *)
-inline_for_extraction
-let vsize_eckem_iv: size_nat = 12
-type eckem_iv_s = lbytes vsize_eckem_iv
-
-(** Definition of a ECKEM counter *)
-type eckem_counter_t = uint32
-
-(** Definition of a ECKEM keys *)
-inline_for_extraction let vsize_eckem_key_asymmetric: size_nat = 32
-type eckem_key_public_s = lbytes vsize_eckem_key_asymmetric
-type eckem_key_private_s = lbytes vsize_eckem_key_asymmetric
+(* BB. TODO: Relocate this constant *)
+let empty : lbytes 0 = create 0 (u8 0)
 
 
-(** Definition of a ECKEM keypair *)
-type eckem_keypair_r = (eckem_key_public_s * option eckem_key_private_s)
+
+(** Constants for ECIES labels *)
+let const_ecies_label_iv : lbytes 8 =
+  [@inline_let]
+  let l = [u8 0x65; u8 0x63; u8 0x69; u8 0x65; u8 0x73; u8 0x20; u8 0x69; u8 0x76] in
+  assert_norm(List.Tot.length l == 8);
+  createL l
+
+let const_ecies_label_key : lbytes 9 =
+  [@inline_let]
+  let l = [u8 0x65; u8 0x63; u8 0x69; u8 0x65; u8 0x73; u8 0x20; u8 0x6b; u8 0x65; u8 0x79] in
+  assert_norm(List.Tot.length l == 9);
+  createL l
+
+
+(** Definition of a ECIES IV *)
+inline_for_extraction let vsize_ecies_iv: size_nat = 12 (* AES_GCM with TLS length IV *)
+
+
+(** Definition of a ECIES keys *)
+inline_for_extraction let vsize_ecies_key_symmetric: size_nat = 16
+inline_for_extraction let vsize_ecies_key_asymmetric: size_nat = 32
+type ecies_key_public_s = lbytes vsize_ecies_key_asymmetric
+type ecies_key_private_s = lbytes vsize_ecies_key_asymmetric
+type ecies_key_s = lbytes vsize_ecies_key_asymmetric
+
+
+(** Definition of a ECIES keypair *)
+type ecies_keypair_r = (ecies_key_public_s * option ecies_key_private_s)
 
 
 (** Generation of an EC public private keypair for Curve25519 *)
-val eckem_secret_to_public: eckem_key_private_s -> Tot eckem_key_public_s
-let eckem_secret_to_public kpriv =
-  let basepoint_zeros = create 32 (u8 0) in
-  let basepoint = upd basepoint_zeros 31 (u8 0x09) in
+val ecies_secret_to_public: ecies_key_private_s -> Tot ecies_key_public_s
+let ecies_secret_to_public kpriv =
+  let basepoint_zeros = create vsize_ecies_key_asymmetric (u8 0) in
+  let basepoint = upd basepoint_zeros (vsize_ecies_key_asymmetric - 1) (u8 0x09) in
   Spec.Curve25519.scalarmult kpriv basepoint
 
 
 (** Generation of an EC public private keypair for Curve25519 *)
-val eckem_generate: unit -> Tot eckem_keypair_r
-let eckem_generate () =
-  let basepoint_zeros = create 32 (u8 0) in
-  let basepoint = upd basepoint_zeros 31 (u8 0x09) in
-  let kpriv = crypto_random vsize_eckem_key_asymmetric in
-  let kpub = eckem_secret_to_public kpriv in
+val ecies_generate: unit -> Tot ecies_keypair_r
+let ecies_generate () =
+  let basepoint_zeros = create vsize_ecies_key_asymmetric (u8 0) in
+  let basepoint = upd basepoint_zeros (vsize_ecies_key_asymmetric - 1) (u8 0x09) in
+  let kpriv = crypto_random vsize_ecies_key_asymmetric in
+  let kpub = ecies_secret_to_public kpriv in
   kpub, Some kpriv
 
 
-(** ECKEM Encryption *)
+(** ECIES Encryption *)
 val encrypt:
     #olen: size_nat
-  -> receiver: eckem_key_public_s
-  -> sender: eckem_key_private_s
-  -> len: size_nat
-  -> input: lbytes len ->
+  -> a: Hash.algorithm
+  -> receiver: ecies_key_public_s
+  -> sender: ecies_key_private_s
+  -> input: bytes ->
   Tot (lbytes olen)
 
-let encrypt #olen receiver sender len input =
-  let kdf_iv = crypto_random vsize_eckem_iv in
-  let ek: lbytes 32 = Spec.Curve25519.scalarmult receiver sender in
+let encrypt #olen a receiver sender input =
+  let len = length input in
+  let ek: lbytes vsize_ecies_key_asymmetric = Spec.Curve25519.scalarmult receiver sender in
   let unsafe = for_all (fun a -> uint_to_nat #U8 a = 0) ek in
-  let stream = Spec.HKDF.hkdf_extract Spec.Hash.SHA2_256 vsize_eckem_iv kdf_iv 32 ek in
-  let key = sub stream 0 Spec.AESGCM.keylen in
-  let iv = sub stream Spec.AESGCM.keylen 12 in
-  let c = Spec.AESGCM.aead_encrypt key 12 iv len input 0 empty in
-  let zeros = create (len + vsize_eckem_iv) (u8 0) in
-  let out = create (len + vsize_eckem_iv) (u8 0) in
-  let out = update_sub out 0 vsize_eckem_iv iv in
-  let out = update_sub out vsize_eckem_iv len c in
+  let kdf_iv_zeros = create vsize_ecies_key_asymmetric (u8 0) in
+  let extracted = Spec.HKDF.hkdf_extract a kdf_iv_zeros ek in
+  let iv = Spec.HKDF.hkdf_expand a extracted const_ecies_label_iv vsize_ecies_iv in
+  let key = Spec.HKDF.hkdf_expand a extracted const_ecies_label_key vsize_ecies_key_symmetric in
+  let out = Spec.AESGCM.aead_encrypt key vsize_ecies_iv iv len input 0 empty in
+  let zeros = create (len + vsize_ecies_iv) (u8 0) in
   if unsafe then zeros else out
 
 
-(** ECKEM Decryption *)
+(** ECIES Decryption *)
 val decrypt:
     #olen: size_nat
-  -> sender: eckem_key_public_s
-  -> receiver: eckem_key_private_s
-  -> len: size_nat
-  -> input: lbytes len ->
+  -> a: Hash.algorithm
+  -> sender: ecies_key_public_s
+  -> receiver: ecies_key_private_s
+  -> input: bytes ->
   Tot (lbytes olen)
 
-let decrypt #olen sender receiver len input =
-  let kdf_iv = sub input 0 vsize_eckem_iv in
-  let ek: lbytes 32 = Spec.Curve25519.scalarmult sender receiver in
+let decrypt #olen a sender receiver input =
+  let len = length input in
+  let ek: lbytes vsize_ecies_key_asymmetric = Spec.Curve25519.scalarmult receiver sender in
   let unsafe = for_all (fun a -> uint_to_nat #U8 a = 0) ek in
-  let stream = Spec.HKDF.hkdf_extract Spec.Hash.SHA2_256 vsize_eckem_iv kdf_iv 32 ek in
-  let key = sub stream 0 Spec.AESGCM.keylen in
-  let iv = sub stream Spec.AESGCM.keylen 12 in
-  let ciphertext = sub input vsize_eckem_iv (len - vsize_eckem_iv) in
-  let out = Spec.AESGCM.aead_decrypt key 12 iv len ciphertext 0 empty in
-  let zeros = create (len + vsize_eckem_iv) (u8 0) in
-  if unsafe then zeros else out
-
-
-///
-/// Alternative API
-///
-
-
-(** ECKEM Encryption *)
-val encrypt_explicit_iv:
-    #olen: size_nat
-  -> iv: eckem_iv_s
-  -> receiver: eckem_key_public_s
-  -> sender: eckem_key_private_s
-  -> len: size_nat
-  -> input: lbytes len ->
-  Tot (lbytes olen)
-
-let encrypt_explicit_iv #olen kdf_iv receiver sender len input =
-  let ek: lbytes 32 = Spec.Curve25519.scalarmult receiver sender in
-  let unsafe = for_all (fun a -> uint_to_nat #U8 a = 0) ek in
-  let stream = Spec.HKDF.hkdf_extract Spec.Hash.SHA2_256 vsize_eckem_iv kdf_iv 32 ek in
-  let key = sub stream 0 Spec.AESGCM.keylen in
-  let iv = sub stream Spec.AESGCM.keylen 12 in
-  let c = Spec.AESGCM.aead_encrypt key 12 iv len input 0 empty in
-  let zeros = create (len + vsize_eckem_iv) (u8 0) in
-  let out = create (len + vsize_eckem_iv) (u8 0) in
-  let out = update_sub out 0 vsize_eckem_iv iv in
-  let out = update_sub out vsize_eckem_iv len c in
-  if unsafe then zeros else out
-
-
-(** ECKEM Decryption *)
-val decrypt_explicit_iv:
-    #olen: size_nat
-  -> iv: eckem_iv_s
-  -> sender: eckem_key_public_s
-  -> receiver: eckem_key_private_s
-  -> len: size_nat
-  -> input: lbytes len ->
-  Tot (lbytes olen)
-
-let decrypt_explicit_iv #olen iv sender receiver len input =
-  let kdf_iv = sub input 0 vsize_eckem_iv in
-  let ek: lbytes 32 = Spec.Curve25519.scalarmult sender receiver in
-  let unsafe = for_all (fun a -> uint_to_nat #U8 a = 0) ek in
-  let stream = Spec.HKDF.hkdf_extract Spec.Hash.SHA2_256 vsize_eckem_iv kdf_iv 32 ek in
-  let key = sub stream 0 Spec.AESGCM.keylen in
-  let iv = sub stream Spec.AESGCM.keylen 12 in
-  let encrypted_plaintext = sub input vsize_eckem_iv (len - vsize_eckem_iv) in
+  let kdf_iv_zeros = create vsize_ecies_key_asymmetric (u8 0) in
+  let extracted = Spec.HKDF.hkdf_extract a kdf_iv_zeros ek in
+  let iv = Spec.HKDF.hkdf_expand a extracted const_ecies_label_iv vsize_ecies_iv in
+  let key = Spec.HKDF.hkdf_expand a extracted const_ecies_label_key vsize_ecies_key_symmetric in
   let out = Spec.AESGCM.aead_decrypt key 12 iv len input 0 empty in
-  let zeros = create (len + vsize_eckem_iv) (u8 0) in
+  let zeros = create (len + vsize_ecies_iv) (u8 0) in
   if unsafe then zeros else out
 
 
@@ -155,22 +122,22 @@ let decrypt_explicit_iv #olen iv sender receiver len input =
 /// which remains to be proven correct.
 ///
 
-(** ECKEM Encryption *)
+(** ECIES Encryption *)
 assume val encrypt_counter:
     #olen: size_nat
-  -> i: eckem_counter_t
-  -> receiver: eckem_key_public_s
-  -> sender: eckem_key_private_s
+  -> i: size_nat
+  -> receiver: ecies_key_public_s
+  -> sender: ecies_key_private_s
   -> len: size_nat
   -> plaintext: lbytes len ->
   Tot (lbytes olen)
 
-(** ECKEM Decryption *)
+(** ECIES Decryption *)
 assume val decrypt_counter:
     #olen: size_nat
-  -> i: eckem_counter_t
-  -> sender: eckem_key_public_s
-  -> receiver: eckem_key_private_s
+  -> i: size_nat
+  -> sender: ecies_key_public_s
+  -> receiver: ecies_key_private_s
   -> len: size_nat
   -> ciphertext: lbytes len ->
   Tot (lbytes olen)
